[Parikh] add comments and reorder lemmas into multiple files

Parikh/Pilling.thy
@@ -1,605 +1,16 @@
-theory Parikh
+theory Pilling
   imports 
     "../CFG"
     "../CFL"
+    "./Lfun"
+    "./Parikh_Img"
     "$AFP/Regular-Sets/Regular_Set"
     "$AFP/Regular-Sets/Regular_Exp"
 begin
 
-
-section \<open>General stuff\<close>
-
-lemma langpow_mono:
-  fixes A :: "'a lang"
-  assumes "A \<subseteq> B"
-  shows "A ^^ n \<subseteq> B ^^ n"
-using assms conc_mono[of A B] by (induction n) auto
-
-
-lemma countable_union_finally_empty:
-  assumes "\<forall>j>i. f j = {}"
-  shows "(\<Union>j. f j) = (\<Union>j\<le>i. f j)"
-  sorry
-
-
-(* currently not needed *)
-lemma generalized_arden: "lfp (\<lambda>X. A @@ X \<union> B) = star A @@ B" (is "lfp ?f = _")
-proof (rule lfp_eqI)
-  show "mono ?f" by (simp add: Un_commute conc_mono le_supI2 monoI)
-
-  have "A @@ star A \<union> {[]} = star A" using star_unfold_left by blast
-  then show "A @@ star A @@ B \<union> B = star A @@ B"
-    by (metis conc_Un_distrib(2) conc_assoc conc_epsilon(1))
-
-  show "\<And>X. A @@ X \<union> B = X \<Longrightarrow> star A @@ B \<subseteq> X"
-  proof -
-    fix X
-    assume "A @@ X \<union> B = X"
-    then have "X = A ^^ Suc n @@ X \<union> (\<Union>m\<le>n. A ^^ m @@ B)" for n using arden_helper by metis
-    then have "A ^^ n @@ B \<subseteq> X" for n by blast
-    then show "star A @@ B \<subseteq> X" unfolding star_def by blast
-  qed
-qed
-
-
-
-section \<open>functions of languages\<close>
-
-datatype 'a lfun = V nat
-                 | N "'a lang"
-                 | Union2 "'a lfun" "'a lfun"
-                 | UnionC "nat \<Rightarrow> 'a lfun"
-                 | Conc "'a lfun" "'a lfun"
-                 | Star "'a lfun"
-
-type_synonym 'a state = "nat \<Rightarrow> 'a lang"
-
-primrec eval :: "'a lfun \<Rightarrow> 'a state \<Rightarrow> 'a lang" where
-  "eval (V n) s = s n" |
-  "eval (N l) _ = l" |
-  "eval (Union2 f g) s = eval f s \<union> eval g s" |
-  "eval (UnionC f) s = (\<Union>i. eval (f i) s)" |
-  "eval (Conc f g) s = eval f s @@ eval g s" |
-  "eval (Star f) s = star (eval f s)"
-
-primrec vars :: "'a lfun \<Rightarrow> nat set" where
-  "vars (V n) = {n}" |
-  "vars (N _) = {}" |
-  "vars (Union2 f g) = vars f \<union> vars g" |
-  "vars (UnionC f) = (\<Union>i. vars (f i))" |
-  "vars (Conc f g) = vars f \<union> vars g" |
-  "vars (Star f) = vars f"
-
-primrec subst :: "'a lfun \<Rightarrow> (nat \<Rightarrow> 'a lfun) \<Rightarrow> 'a lfun" where
-  "subst (V n) s = s n" |
-  "subst (N l) _ = N l" |
-  "subst (Union2 f g) s = Union2 (subst f s) (subst g s)" |
-  "subst (UnionC f) s = UnionC (\<lambda>i. subst (f i) s)" |
-  "subst (Conc f g) s = Conc (subst f s) (subst g s)" |
-  "subst (Star f) s = Star (subst f s)"
-
-
-lemma lfun_mono_aux:
-  assumes "\<forall>i. s i \<subseteq> s' i"
-    shows "eval f s \<subseteq> eval f s'"
-using assms proof (induction rule: lfun.induct)
-  case (Conc x1a x2a)
-  then show ?case by fastforce
-next
-  case (Star f)
-  then show ?case
-    by (smt (verit, best) eval.simps(6) in_star_iff_concat order_trans subsetI)
-qed auto
-
-lemma lfun_mono:
-  fixes f :: "'a lfun"
-  shows "mono (eval f)"
-  using lfun_mono_aux by (metis le_funD monoI)
-
-
-lemma substitution_lemma:
-  assumes "\<forall>i. s' i = eval (upd i) s"
-  shows "eval (subst f upd) s = eval f s'"
-  using assms by (induction rule: lfun.induct) auto
-
-
-lemma vars_subst: "vars (subst f upd) = (\<Union>x \<in> vars f. vars (upd x))"
-  by (induction f) auto
-
-lemma vars_subst_upper: "vars (subst f upd) \<subseteq> (\<Union>x. vars (upd x))"
-  using vars_subst by force
-
-
-lemma eval_vars:
-  assumes "\<forall>i \<in> vars f. s i = s' i"
-  shows "eval f s = eval f s'"
-  using assms by (induction f) auto
-
-lemma eval_vars_subst:
-  assumes "\<forall>i \<in> vars f. s i = eval (upd i) s"
-  shows "eval (subst f upd) s = eval f s"
-proof -
-  let ?s' = "\<lambda>i. if i \<in> vars f then s i else eval (upd i) s"
-  let ?s'' = "\<lambda>i. eval (upd i) s"
-  have s'_s'': "?s' i = ?s'' i" for i using assms by simp
-  then have s_s'': "\<forall>i. ?s'' i = eval (upd i) s" by simp
-
-  from assms have "eval f s = eval f ?s'" using eval_vars[of f] by simp
-  also have "\<dots> = eval (subst f upd) s"
-    using assms substitution_lemma[OF s_s'', of f] by (simp add: eval_vars)
-  finally show ?thesis by simp
-qed
-
-
-(* Continuity of lfun *)
-
-lemma lfun_cont_aux1:
-  assumes "\<forall>i. s i \<le> s (Suc i)"
-      and "w \<in> (\<Union>i. eval f (s i))"
-    shows "w \<in> eval f (\<lambda>x. \<Union>i. s i x)"
-proof -
-  from assms(2) obtain n where n_intro: "w \<in> eval f (s n)" by auto
-  have "s n x \<subseteq> (\<Union>i. s i x)" for x by auto
-  with n_intro show "?thesis"
-    using lfun_mono_aux[of "s n" "\<lambda>x. \<Union>i. s i x"] by auto
-qed
-
-lemma langpow_Union_eval:
-  assumes "\<forall>i. s i \<le> s (Suc i)"
-      and "w \<in> (\<Union>i. eval f (s i)) ^^ n"
-    shows "w \<in> (\<Union>i. eval f (s i) ^^ n)"
-using assms proof (induction n arbitrary: w)
-  case 0
-  then show ?case by simp
-next
-  case (Suc n)
-  then obtain u v where w_decomp: "w = u@v" and
-    "u \<in> (\<Union>i. eval f (s i)) \<and> v \<in> (\<Union>i. eval f (s i)) ^^ n" by fastforce
-  with Suc have "u \<in> (\<Union>i. eval f (s i)) \<and> v \<in> (\<Union>i. eval f (s i) ^^ n)" by auto
-  then obtain i j where i_intro: "u \<in> eval f (s i)" and j_intro: "v \<in> eval f (s j) ^^ n" by blast
-  let ?m = "max i j"
-  from i_intro Suc.prems(1) lfun_mono_aux have 1: "u \<in> eval f (s ?m)"
-    by (metis le_fun_def lift_Suc_mono_le max.cobounded1 subset_eq)
-  from Suc.prems(1) lfun_mono_aux have "eval f (s j) \<subseteq> eval f (s ?m)"
-    by (metis le_fun_def lift_Suc_mono_le max.cobounded2)
-  with j_intro langpow_mono have 2: "v \<in> eval f (s ?m) ^^ n" by auto
-  from 1 2 show ?case using w_decomp by auto
-qed
-
-lemma lfun_cont_aux2:
-  assumes "\<forall>i. s i \<le> s (Suc i)"
-      and "w \<in> eval f (\<lambda>x. \<Union>i. s i x)"
-    shows "w \<in> (\<Union>i. eval f (s i))"
-using assms proof (induction arbitrary: w rule: lfun.induct)
-  case (Conc f g)
-  then obtain u v where w_decomp: "w = u@v"
-    and "u \<in> eval f (\<lambda>x. \<Union>i. s i x) \<and> v \<in> eval g (\<lambda>x. \<Union>i. s i x)" by auto
-  with Conc have "u \<in> (\<Union>i. eval f (s i)) \<and> v \<in> (\<Union>i. eval g (s i))" by auto
-  then obtain i j where i_intro: "u \<in> eval f (s i)" and j_intro: "v \<in> eval g (s j)" by blast
-  let ?m = "max i j"
-  from i_intro Conc.prems(1) lfun_mono_aux have "u \<in> eval f (s ?m)"
-    by (metis le_fun_def lift_Suc_mono_le max.cobounded1 subset_eq)
-  moreover from j_intro Conc.prems(1) lfun_mono_aux have "v \<in> eval g (s ?m)"
-    by (metis le_fun_def lift_Suc_mono_le max.cobounded2 subset_eq)
-  ultimately show ?case using w_decomp by auto
-next
-  case (Star f)
-  then obtain n where n_intro: "w \<in> (eval f (\<lambda>x. \<Union>i. s i x)) ^^ n"
-    using eval.simps(6) star_pow by blast
-  with Star have "w \<in> (\<Union>i. eval f (s i)) ^^ n" using langpow_mono by blast
-  with Star.prems have "w \<in> (\<Union>i. eval f (s i) ^^ n)" using langpow_Union_eval by auto
-  then show ?case by (auto simp add: star_def)
-qed fastforce+
-
-lemma lfun_cont:
-  assumes "\<forall>i. s i \<le> s (Suc i)"
-  shows "eval f (\<lambda>x. \<Union>i. s i x) = (\<Union>i. eval f (s i))"
-proof
-  from assms show "eval f (\<lambda>x. \<Union>i. s i x) \<subseteq> (\<Union>i. eval f (s i))" using lfun_cont_aux2 by auto
-  from assms show "(\<Union>i. eval f (s i)) \<subseteq> eval f (\<lambda>x. \<Union>i. s i x)" using lfun_cont_aux1 by blast
-qed
-
-
-
-section \<open>Regular functions\<close>
-
-inductive regular_fun :: "'a lfun \<Rightarrow> bool" where
-  Variable:    "regular_fun (V _)" |
-  Const:       "regular_lang l \<Longrightarrow> regular_fun (N l)" |
-  Union2:      "\<lbrakk> regular_fun f; regular_fun g \<rbrakk> \<Longrightarrow> regular_fun (Union2 f g)" |
-  Conc:        "\<lbrakk> regular_fun f; regular_fun g \<rbrakk> \<Longrightarrow> regular_fun (Conc f g)" |
-  Star:        "regular_fun f \<Longrightarrow> regular_fun (Star f)"
-
-declare regular_fun.intros [intro]
-inductive_cases ConstE [elim]:       "regular_fun (N l)"
-inductive_cases Union2E [elim]:      "regular_fun (Union2 f g)"
-inductive_cases ConcE [elim]:        "regular_fun (Conc f g)"
-inductive_cases StarE [elim]:        "regular_fun (Star f)"
-
-
-lemma finite_union_regular:
-  assumes "\<forall>j\<le>i. regular_fun (f j)"
-      and "\<forall>j>i. f j = N {}"
-    shows "\<exists>g. regular_fun g \<and> (\<forall>s. eval (UnionC f) s = eval g s)"
-using assms proof (induction i arbitrary: f)
-  case 0
-  then have "eval (UnionC f) s = eval (f 0) s" for s
-    using countable_union_finally_empty[of 0 "\<lambda>j. eval (f j) s"] by simp
-  with "0.prems" show ?case by blast
-next
-  case (Suc i)
-  let ?f' = "(\<lambda>j. if j \<le> i then f j else N {})"
-  from Suc obtain g' where "regular_fun g' \<and> (\<forall>s. eval (UnionC ?f') s = eval g' s)" by fastforce
-  moreover with Suc.prems have "eval (UnionC f) s = eval (Union2 g' (f (Suc i))) s" for s
-    using countable_union_finally_empty[of "Suc i" "\<lambda>j. eval (f j) s"]
-          countable_union_finally_empty[of i "\<lambda>j. eval (?f' j) s"]
-    by (simp add: atMost_Suc sup_commute)
-  ultimately show ?case using Suc.prems by blast
-qed
-
-
-lemma regular_fun_regular:
-  assumes "regular_fun f"
-      and "\<And>n. n \<in> vars f \<Longrightarrow> regular_lang (s n)"
-    shows "regular_lang (eval f s)"
-using assms proof (induction rule: regular_fun.induct)
-  case (Union2 f g)
-  then obtain r1 r2 where "Regular_Exp.lang r1 = eval f s \<and> Regular_Exp.lang r2 = eval g s" by auto
-  then have "Regular_Exp.lang (Plus r1 r2) = eval (Union2 f g) s" by simp
-  then show ?case by blast
-next
-  case (Conc f g)
-  then obtain r1 r2 where "Regular_Exp.lang r1 = eval f s \<and> Regular_Exp.lang r2 = eval g s" by auto
-  then have "Regular_Exp.lang (Times r1 r2) = eval (Conc f g) s" by simp
-  then show ?case by blast
-next
-  case (Star f)
-  then obtain r  where "Regular_Exp.lang r = eval f s" by auto
-  then have "Regular_Exp.lang (Regular_Exp.Star r) = eval (Star f) s" by simp
-  then show ?case by blast
-qed auto
-
-
-lemma subst_reg_fun:
-  assumes "regular_fun f"
-      and "\<forall>x \<in> vars f. regular_fun (upd x)"
-    shows "regular_fun (subst f upd)"
-  using assms by (induction rule: regular_fun.induct) auto
-
-
-
-section \<open>Parikh image\<close>
-
-(* Parikh vector *)
-
-definition parikh_vec :: "'t list \<Rightarrow> ('t \<Rightarrow> nat)" where
-  "parikh_vec xs c = length (filter (\<lambda>x. c = x) xs)"
-
-definition vec0 :: "'t \<Rightarrow> nat" where
-  "vec0 c \<equiv> 0"
-
-lemma parikh_vec_concat: "parikh_vec (u@v) = (\<lambda>c. parikh_vec u c + parikh_vec v c)"
-  by (auto simp add: parikh_vec_def)
-
-lemma parikh_vec_commut: "parikh_vec (u@v) = parikh_vec (v@u)"
-  by (auto simp add: parikh_vec_def)
-
-lemma parikh_vec_left_conc: "parikh_vec u = parikh_vec u' \<Longrightarrow> parikh_vec (u@v) = parikh_vec (u'@v)"
-  unfolding parikh_vec_def by (metis filter_append replicate_length_filter)
-
-lemma parikh_vec_right_conc: "parikh_vec u = parikh_vec u' \<Longrightarrow> parikh_vec (v@u) = parikh_vec (v@u')"
-  unfolding parikh_vec_def by (metis filter_append replicate_length_filter)
-
-(* Parikh image *)
-
-definition parikh_img :: "'t lang \<Rightarrow> ('t \<Rightarrow> nat) set" where
-  "parikh_img L = { parikh_vec w | w. w \<in> L }"
-
-(* TODO: really necessary? *)
-definition subseteq_comm :: "'t lang \<Rightarrow> 't lang \<Rightarrow> bool" where
-  "subseteq_comm L1 L2 \<equiv> parikh_img L1 \<subseteq> parikh_img L2"
-
-lemma "w \<in> L \<Longrightarrow> parikh_vec w \<in> parikh_img L"
-  unfolding parikh_img_def by auto
-
-lemma "parikh_vec w \<in> parikh_img L \<Longrightarrow> \<exists>w'. parikh_vec w = parikh_vec w' \<and> w' \<in> L"
-  unfolding parikh_img_def by blast
-
-lemma parikh_img_Un [simp]: "parikh_img (L1 \<union> L2) = parikh_img L1 \<union> parikh_img L2"
-  by (auto simp add: parikh_img_def)
-
-lemma parikh_img_UNION: "parikh_img (\<Union>(L ` I)) = \<Union> ((\<lambda>i. parikh_img (L i)) ` I)"
-  by (auto simp add: parikh_img_def)
-
-lemma parikh_img_mono: "A \<subseteq> B \<Longrightarrow> parikh_img A \<subseteq> parikh_img B"
-  unfolding parikh_img_def by fast
-
-lemma parikh_img_conc: "parikh_img (L1 @@ L2) = { (\<lambda>c. v1 c + v2 c) | v1 v2. v1 \<in> parikh_img L1 \<and> v2 \<in> parikh_img L2 }" (is "_ = ?R")
-proof -
-  have "parikh_img (L1 @@ L2) = { parikh_vec (u@v) | u v. u \<in> L1 \<and> v \<in> L2 }" (is "_ = ?M")
-    using parikh_img_def[of "L1 @@ L2"] conc_def by blast
-  moreover have "?M \<subseteq> ?R"
-    using parikh_vec_concat parikh_img_def by blast
-  moreover have "?R \<subseteq> ?M"
-  proof
-    fix x
-    assume "x \<in> ?R"
-    then obtain v1 v2 where v1_v2: "v1 \<in> parikh_img L1 \<and> v2 \<in> parikh_img L2 \<and> x = (\<lambda>c. v1 c + v2 c)"
-      by auto
-    then obtain u1 u2 where "u1 \<in> L1" "parikh_vec u1 = v1" "u2 \<in> L2" "parikh_vec u2 = v2"
-      using parikh_img_def by (smt (verit) mem_Collect_eq)
-    then show "x \<in> ?M"
-      using parikh_vec_concat[of u1 u2] v1_v2 by force
-  qed
-  ultimately show ?thesis by auto
-qed
-
-lemma parikh_img_commut: "parikh_img (L1 @@ L2) = parikh_img (L2 @@ L1)"
-proof -
-  have "{ (\<lambda>c. v1 c + v2 c) | v1 v2. v1 \<in> parikh_img L1 \<and> v2 \<in> parikh_img L2 } =
-        { (\<lambda>c. v1 c + v2 c) | v1 v2. v1 \<in> parikh_img L2 \<and> v2 \<in> parikh_img L1 }"
-    using add.commute by blast
-  then show ?thesis
-    using parikh_img_conc[of L1] parikh_img_conc[of L2] by auto
-qed
-
-lemma parikh_conc_right_subset: "parikh_img A \<subseteq> parikh_img B \<Longrightarrow> parikh_img (A @@ C) \<subseteq> parikh_img (B @@ C)"
-  by (auto simp add: parikh_img_conc)
-
-lemma parikh_conc_right: "parikh_img A = parikh_img B \<Longrightarrow> parikh_img (A @@ C) = parikh_img (B @@ C)"
-  by (auto simp add: parikh_img_conc)
-
-lemma parikh_conc_left: "parikh_img A = parikh_img B \<Longrightarrow> parikh_img (C @@ A) = parikh_img (C @@ B)"
-  by (auto simp add: parikh_img_conc)
-
-lemma parikh_pow_distrib: "parikh_img A \<subseteq> parikh_img B \<Longrightarrow> parikh_img (A ^^ n) \<subseteq> parikh_img (B ^^ n)"
-  by (induction n) (auto simp add: parikh_img_conc)
-
-lemma parikh_star_distrib:
-  assumes "parikh_img A \<subseteq> parikh_img B"
-  shows "parikh_img (star A) \<subseteq> parikh_img (star B)"
-proof
-  fix v
-  assume "v \<in> parikh_img (star A)"
-  then obtain w where w_intro: "parikh_vec w = v \<and> w \<in> star A" unfolding parikh_img_def by blast
-  then obtain n where "w \<in> A ^^ n" unfolding star_def by blast
-  then have "v \<in> parikh_img (A ^^ n)" using w_intro unfolding parikh_img_def by blast
-  with assms have "v \<in> parikh_img (B ^^ n)" using parikh_pow_distrib by blast
-  then show "v \<in> parikh_img (star B)" unfolding star_def using parikh_img_UNION by fastforce
-qed
-
-lemma parikh_star_distrib_eq:
-  assumes "parikh_img A = parikh_img B"
-  shows "parikh_img (star A) = parikh_img (star B)"
-  using parikh_star_distrib by (metis Orderings.order_eq_iff assms)
-
-lemma parikh_img_union_pow_aux1:
-  assumes "v \<in> parikh_img ((A \<union> B) ^^ n)"
-    shows "v \<in> parikh_img (\<Union>i \<le> n. A ^^ i @@ B ^^ (n-i))"
-using assms proof (induction n arbitrary: v)
-  case 0
-  then show ?case by simp
-next
-  case (Suc n)
-  then obtain w where w_intro: "w \<in> (A \<union> B) ^^ (Suc n) \<and> parikh_vec w = v"
-    unfolding parikh_img_def by auto
-  then obtain w1 w2 where w1_w2_intro: "w = w1@w2 \<and> w1 \<in> A \<union> B \<and> w2 \<in> (A \<union> B) ^^ n" by fastforce
-  let ?v1 = "parikh_vec w1" and ?v2 = "parikh_vec w2"
-
-  from w1_w2_intro have "?v2 \<in> parikh_img ((A \<union> B) ^^ n)" unfolding parikh_img_def by blast
-  with Suc.IH have "?v2 \<in> parikh_img (\<Union>i \<le> n. A ^^ i @@ B ^^ (n-i))" by auto
-  then obtain w2' where w2'_intro: "parikh_vec w2' = parikh_vec w2 \<and>
-      w2' \<in> (\<Union>i \<le> n. A ^^ i @@ B ^^ (n-i))" unfolding parikh_img_def by fastforce
-  then obtain i where i_intro: "i \<le> n \<and> w2' \<in> A ^^ i @@ B ^^ (n-i)" by blast
-
-  from w1_w2_intro w2'_intro have "parikh_vec w = parikh_vec (w1@w2')"
-    using parikh_vec_right_conc by metis
-  moreover have "parikh_vec (w1@w2') \<in> parikh_img (\<Union>i \<le> Suc n. A ^^ i @@ B ^^ (Suc n-i))"
-  proof (cases "w1 \<in> A")
-    case True
-    with i_intro have Suc_i_valid: "Suc i \<le> Suc n" and "w1@w2' \<in> A ^^ (Suc i) @@ B ^^ (Suc n - Suc i)"
-      by (auto simp add: conc_assoc)
-    then have "parikh_vec (w1@w2') \<in> parikh_img (A ^^ (Suc i) @@ B ^^ (Suc n - Suc i))"
-      unfolding parikh_img_def by auto
-    with Suc_i_valid parikh_img_UNION show ?thesis by fast
-  next
-    case False
-    with w1_w2_intro have "w1 \<in> B" by blast
-    with i_intro have "parikh_vec (w1@w2') \<in> parikh_img (B @@ A ^^ i @@ B ^^ (n-i))"
-      unfolding parikh_img_def by blast
-    then have "parikh_vec (w1@w2') \<in> parikh_img (A ^^ i @@ B ^^ (Suc n-i))"
-      using parikh_img_commut conc_assoc
-      by (metis Suc_diff_le conc_pow_comm i_intro lang_pow.simps(2))
-    with i_intro parikh_img_UNION show ?thesis by fastforce
-  qed
-  ultimately show ?case using w_intro by auto
-qed
-
-(*lemma parikh_img_union_pow_aux2:
-  assumes "v \<in> parikh_img (\<Union>i \<le> n. A ^^ i @@ B ^^ (n-i))"
-  shows "v \<in> parikh_img ((A \<union> B) ^^ n)"
-proof -
-  from assms parikh_img_UNION have "v \<in> (\<Union>i\<le>n. parikh_img (A ^^ i @@B ^^ (n-i)))" by metis
-  then obtain i where i_leq_n: "i \<le> n" and "v \<in> parikh_img (A ^^ i @@ B ^^ (n-i))" by blast
-  then obtain w where w_intro: "parikh_vec w = v \<and> w \<in> A ^^ i @@ B ^^ (n-i)"
-    unfolding parikh_img_def by blast
-  then have "w \<in> (A \<union> B) ^^ i @@ B ^^ (n-i)" by (meson conc_mono langpow_mono subset_eq sup_ge1)
-  then have "w \<in> (A \<union> B) ^^ i @@ (A \<union> B) ^^ (n-i)" by (meson conc_mono langpow_mono subset_eq sup_ge2)
-  then have "w \<in> (A \<union> B) ^^ n" using lang_pow_add[of "i" "n-i" "A\<union>B"] i_leq_n by simp
-  then show ?thesis using w_intro unfolding parikh_img_def by blast
-qed*)
-
-lemma parikh_img_star_aux1:
-  assumes "v \<in> parikh_img (star (A \<union> B))"
-  shows "v \<in> parikh_img (star A @@ star B)"
-proof -
-  from assms have "v \<in> (\<Union>n. parikh_img ((A \<union> B) ^^ n))"
-    unfolding star_def using parikh_img_UNION by metis
-  then obtain n where "v \<in> parikh_img ((A \<union> B) ^^ n)" by blast
-  then have "v \<in> parikh_img (\<Union>i \<le> n. A ^^ i @@ B ^^ (n-i))"
-    using parikh_img_union_pow_aux1 by auto
-  then have "v \<in> (\<Union>i\<le>n. parikh_img (A ^^ i @@ B ^^ (n-i)))" using parikh_img_UNION by metis
-  then obtain i where "i\<le>n \<and> v \<in> parikh_img (A ^^ i @@ B ^^ (n-i))" by blast
-  then obtain w where w_intro: "parikh_vec w = v \<and> w \<in> A ^^ i @@ B ^^ (n-i)"
-    unfolding parikh_img_def by blast
-  then obtain w1 w2 where w_decomp: "w=w1@w2 \<and> w1 \<in> A ^^ i \<and> w2 \<in> B ^^ (n-i)" by blast
-  then have "w1 \<in> star A" and "w2 \<in> star B" by auto
-  with w_decomp have "w \<in> star A @@ star B" by auto
-  with w_intro show ?thesis unfolding parikh_img_def by blast
-qed
-
-lemma parikh_img_star_aux2:
-  assumes "v \<in> parikh_img (star A @@ star B)"
-  shows "v \<in> parikh_img (star (A \<union> B))"
-proof -
-  from assms obtain w where w_intro: "parikh_vec w = v \<and> w \<in> star A @@ star B"
-    unfolding parikh_img_def by blast
-  then obtain w1 w2 where w_decomp: "w=w1@w2 \<and> w1 \<in> star A \<and> w2 \<in> star B" by blast
-  then obtain i j where "w1 \<in> A ^^ i" and w2_intro: "w2 \<in> B ^^ j" unfolding star_def by blast
-  then have w1_in_union: "w1 \<in> (A \<union> B) ^^ i" using langpow_mono by blast
-  from w2_intro have "w2 \<in> (A \<union> B) ^^ j" using langpow_mono by blast
-  with w1_in_union w_decomp have "w \<in> (A \<union> B) ^^ (i+j)" using lang_pow_add by fast
-  with w_intro show ?thesis unfolding parikh_img_def by auto
-qed
-
-lemma parikh_img_star: "parikh_img (star (A \<union> B)) = parikh_img (star A @@ star B)"
-proof
-  show "parikh_img (star (A \<union> B)) \<subseteq> parikh_img (star A @@ star B)" using parikh_img_star_aux1 by auto
-  show "parikh_img (star A @@ star B) \<subseteq> parikh_img (star (A \<union> B))" using parikh_img_star_aux2 by auto
-qed
-
-
-lemma parikh_img_star2: "parikh_img (star (star E @@ F)) = parikh_img ({[]} \<union> star E @@ star F @@ F)"
-  sorry
-
-
-lemma parikh_img_arden_aux:
-  assumes "parikh_img (A @@ X \<union> B) \<subseteq> parikh_img X"
-  shows "parikh_img (A ^^ n @@ B) \<subseteq> parikh_img X"
-using assms proof (induction n)
-  case 0
-  then show ?case by auto
-next
-  case (Suc n)
-  then have "parikh_img (A ^^ (Suc n) @@ B) \<subseteq> parikh_img (A @@ A ^^ n @@B)"
-    by (simp add: conc_assoc)
-  moreover from Suc parikh_conc_left have "\<dots> \<subseteq> parikh_img (A @@ X)"
-    by (metis conc_Un_distrib(1) parikh_img_Un sup.orderE sup.orderI)
-  moreover from Suc.prems have "\<dots> \<subseteq> parikh_img X" by auto
-  ultimately show ?case by fast
-qed
-
-lemma parikh_img_arden:
-  assumes "parikh_img (A @@ X \<union> B) \<subseteq> parikh_img X"
-  shows "parikh_img (star A @@ B) \<subseteq> parikh_img X"
-proof
-  fix x
-  assume "x \<in> parikh_img (star A @@ B)"
-  then have "\<exists>n. x \<in> parikh_img (A ^^ n @@ B)"
-    unfolding star_def by (simp add: conc_UNION_distrib(2) parikh_img_UNION)
-  then obtain n where "x \<in> parikh_img (A ^^ n @@ B)" by blast
-  then show "x \<in> parikh_img X" using parikh_img_arden_aux[OF assms] by fast
-qed
-
-
-(* Pilling's paper shows "=", but needs an additional assumption and I don't unterstand how
-   the proof should work in the Union case:
-     if f(Y*Z, X\<^sub>1, \<dots>, X\<^sub>m) = g(Y*Z, X\<^sub>1, \<dots>, X\<^sub>m) \<union> h(Y*Z, X\<^sub>1, \<dots>, X\<^sub>m) and g contains Y*Z, but h doesn't,
-     then g(Y*Z, X\<^sub>1, \<dots>, X\<^sub>m) \<union> h(Y*Z, X\<^sub>1, \<dots>, X\<^sub>m) = Y* (g(Z, X\<^sub>1, \<dots>, X\<^sub>m) \<union> h(Z, X\<^sub>1, \<dots>, X\<^sub>m)) seems
-     wrong to me
- *)
-lemma reg_fun_homogeneous_aux:
-  assumes "regular_fun f"
-      and "s x = star Y @@ Z"
-    shows "eval f s \<subseteq> star Y @@ eval f (s(x := Z))"
-using assms proof (induction rule: regular_fun.induct)
-  case (Variable uu)
-  then show ?case sorry
-next
-  case (Const l)
-  have "eval (N l) s \<subseteq> star Y @@ eval (N l) s" using concI_if_Nil1 by blast
-  then show ?case by simp
-next
-  case (Union2 f g)
-  then show ?case sorry
-next
-  case (Conc f g)
-  then show ?case sorry
-next
-  case (Star f)
-  then show ?case sorry
-qed
-
-lemma reg_fun_homogeneous:
-  assumes "regular_fun f"
-      and "regular_fun y"
-      and "regular_fun z"
-    shows "eval (subst f (\<lambda>a. if a = x then Conc (Star y) z else V a)) s
-      \<subseteq> eval (Conc (Star y) (subst f (\<lambda>a. if a = x then z else V a))) s" (is "?L \<subseteq> ?R")
-proof -
-  let ?s' = "\<lambda>a. if a = x then star (eval y s) @@ eval z s else s a"
-  have "?L = eval f ?s'"
-    using substitution_lemma[of ?s' "\<lambda>a. if a = x then Conc (Star y) z else V a"] by fastforce
-  also have "\<dots> \<subseteq> star (eval y s) @@ eval f (?s'(x := eval z s))"
-    using assms reg_fun_homogeneous_aux[of f ?s'] by simp
-  also have "\<dots> = ?R" using substitution_lemma[of "?s'(x := eval z s)"] by simp
-  finally show ?thesis .
-qed
-
-(* Proof sketch
-
-f(Y*Z, X1, \<dots>, Xm) \<subseteq> Y* f(Z, X1, \<dots>, Xm)
-
-Case f = g \<union> h:
-  if Y*Z \<in> g and h: g(Y*Z, X1, \<dots>, Xm) \<union> h(Y*Z, X1, \<dots>, Xm) = Y* g(Z, X1, \<dots>, Xm) \<union> Y* h(Z, X1, \<dots>, Xm)
-    = Y* f(Z, X1, \<dots>, Xm)
-  if Y*Z \<in> g, but not in h: g(Y*Z, X1, \<dots>, Xm) \<union> h(X1, \<dots>, Xm) = Y* g(Z, X1, \<dots>, Xm) \<union> h(X1, \<dots>, Xm)
-    = 
-
-Case f = g h:
-  if Y*Z \<in> g and h: g(Y*Z, \<dots>) h(Y*Z, \<dots>) = Y* g(Z, \<dots>) Y* h(Z, \<dots>) = Y* f(Z, \<dots>)
-  if Y*Z \<in> g, but not in h: g(Y*Z) h(\<dots>) = Y* g(Z) h(\<dots>) = Y* f(Z, \<dots>)
-
-Case f = Star g
-  g(Y*Z)* = (Y* g(Z))* = Y* g(Z)*
-
-*)
-
-
-lemma parikh_img_subst_mono:
-  assumes "\<forall>i. parikh_img (eval (A i) s) \<subseteq> parikh_img (eval (B i) s)"
-  shows "parikh_img (eval (subst f (\<lambda>i. A i)) s) \<subseteq> parikh_img (eval (subst f (\<lambda>i. B i)) s)"
-  sorry
-
-lemma parikh_img_subst_mono_eq:
-  assumes "\<forall>i. parikh_img (eval (A i) s) = parikh_img (eval (B i) s)"
-  shows "parikh_img (eval (subst f (\<lambda>i. A i)) s) = parikh_img (eval (subst f (\<lambda>i. B i)) s)"
-  using parikh_img_subst_mono assms by blast
-
-
-section \<open>functions of parikh images\<close>
-
-type_synonym 'a plang = "('a \<Rightarrow> nat) set"
-
-datatype 'a pfun = V' nat
-                 | N' "'a plang"
-                 | Union2' "'a pfun" "'a pfun"
-                 | Conc' "'a pfun" "'a pfun"
-                 | Star' "'a pfun"
-
-type_synonym 'a pstate = "nat \<Rightarrow> 'a plang"
-
-(*fun eval' :: "'a pfun \<Rightarrow> 'a pstate \<Rightarrow> 'a plang" where
-  "eval' (V' n) s = s n" |
-  "eval' (N' l) _ = l" |
-  "eval' (Union2' f g) s = eval' f s \<union> eval' g s" |
-  "eval' (Conc' f g) s = { (\<lambda>c. v1 c + v2 c) | v1 v2. v1 \<in> eval' f s \<and> v2 \<in> eval' g s }" |
-  "eval' (Star f) s = star (eval f s)"*)
-
-
-
 section \<open>systems of equations\<close>
 
+(* We just represent the right hand sides *)
 type_synonym 'a eq_sys = "'a lfun list"
 
 (* sys independent on variables \<le> n *)
@@ -610,48 +21,53 @@ definition indep_ub :: "'a eq_sys \<Rightarrow> nat \<Rightarrow> bool" where
 definition indep_lb :: "'a eq_sys \<Rightarrow> nat \<Rightarrow> bool" where
   "indep_lb sys n \<equiv> \<forall>eq \<in> set sys. \<forall>x \<in> vars eq. x < n"
 
+(* solves equation with \<subseteq> *)
 definition solves_ineq_sys :: "'a eq_sys \<Rightarrow> 'a state \<Rightarrow> bool" where
   "solves_ineq_sys sys s \<equiv> \<forall>i < length sys. eval (sys ! i) s \<subseteq> s i"
 
+(* solves equation with = *)
 definition solves_eq_sys :: "'a eq_sys \<Rightarrow> 'a state \<Rightarrow> bool" where
   "solves_eq_sys sys s \<equiv> \<forall>i < length sys. eval (sys ! i) s = s i"
 
+(* solves equation with \<subseteq>, only caring about the Parikh image *)
 definition solves_ineq_comm :: "nat \<Rightarrow> 'a lfun \<Rightarrow> 'a state \<Rightarrow> bool" where
   "solves_ineq_comm x eq s \<equiv> parikh_img (eval eq s) \<subseteq> parikh_img (s x)"
 
+(* solves equation system with \<subseteq>, only caring about the Parikh image *)
 definition solves_ineq_sys_comm :: "'a eq_sys \<Rightarrow> 'a state \<Rightarrow> bool" where
   "solves_ineq_sys_comm sys s \<equiv> \<forall>i < length sys. solves_ineq_comm i (sys ! i) s"
 
+(* solves equation with =, only caring about the Parikh image*)
 definition solves_eq_comm :: "nat \<Rightarrow> 'a lfun \<Rightarrow> 'a state \<Rightarrow> bool" where
   "solves_eq_comm x eq s \<equiv> parikh_img (eval eq s) = parikh_img (s x)"
 
+(* solves equation system with =, only caring about the Parikh image *)
 definition solves_eq_sys_comm :: "'a eq_sys \<Rightarrow> 'a state \<Rightarrow> bool" where
   "solves_eq_sys_comm sys s \<equiv> \<forall>i < length sys. solves_eq_comm i (sys ! i) s"
 
+(* Substituion into each equation of a system *)
 definition sys_subst :: "'a eq_sys \<Rightarrow> (nat \<Rightarrow> 'a lfun) \<Rightarrow> 'a eq_sys" where
   "sys_subst sys s \<equiv> map (\<lambda>eq. subst eq s) sys"
 
+(* partial solution with \<subseteq>, only caring about the Parikh image *)
 definition partial_sol_ineq :: "nat \<Rightarrow> 'a lfun \<Rightarrow> 'a lfun \<Rightarrow> bool" where
   "partial_sol_ineq x eq sol \<equiv> (\<forall>s.
     parikh_img (eval (subst eq (\<lambda>i. if i = x then sol else V i)) s) \<subseteq> parikh_img (eval sol s)
   )"
 
+(* partial solution with =, only caring about the Parikh image *)
 definition partial_sol_eq :: "nat \<Rightarrow> 'a lfun \<Rightarrow> 'a lfun \<Rightarrow> bool" where
   "partial_sol_eq x eq sol \<equiv> (\<forall>s.
     parikh_img (eval (subst eq (\<lambda>i. if i = x then sol else V i)) s) = parikh_img (eval sol s)
   )"
 
+(* minimal (partial) solution of a single equation with = *)
 definition partial_min_reg_sol_eq :: "nat \<Rightarrow> 'a lfun \<Rightarrow> 'a lfun \<Rightarrow> bool" where
   "partial_min_reg_sol_eq x eq sol \<equiv>
     regular_fun sol \<and> x \<notin> vars sol \<and> partial_sol_eq x eq sol
       \<and> (\<forall>sol'. x \<notin> vars sol' \<and> partial_sol_ineq x eq sol'
                 \<longrightarrow> (\<forall>s. parikh_img (eval sol s) \<subseteq> parikh_img (eval sol' s)))"
 
-(* wrong *)
-(* definition partial_sol_eq_sys :: "'a eq_sys \<Rightarrow> 'a eq_sys \<Rightarrow> bool" where
-  "partial_sol_eq_sys sys sol \<equiv> length sol = length sys \<and> indep_ub sol (length sys - 1)
-        \<and> (\<forall>s. solves_eq_sys_comm (sys_subst sys (\<lambda>i. if i < length sys then sol ! i else V i)) s)"
-*)
 
 lemma partial_sol_ineq_solves_ineq_comm:
   "partial_sol_ineq x eq sol \<longleftrightarrow> (\<forall>s. solves_ineq_comm x eq (s(x := eval sol s)))"
@@ -683,7 +99,17 @@ proof
 qed
 
 
-section \<open>The lemma from the paper\<close>
+
+section \<open>The lemma from Pilling's paper\<close>
+
+(* In this section, the lemma from Pilling's paper will be proved.
+   For some reason, the lemma will not be needed in the further proof.
+*)
+
+locale pillings_lemma
+begin
+
+subsection \<open>g_pre (in the paper g_{iN} resp. X_{iN}\<close>
 
 fun g_pre :: "'a eq_sys \<Rightarrow> nat \<Rightarrow> nat \<Rightarrow> 'a lfun" where
   "g_pre _ _ 0 = N {}" |
@@ -756,6 +182,10 @@ next
 qed
 
 
+
+subsection \<open>g\<close>
+
+(* This is the only reason why we have included the countable union in the lfun definition *)
 definition g :: "'a eq_sys \<Rightarrow> nat \<Rightarrow> 'a lfun" where
   "g f_sys i \<equiv> UnionC (\<lambda>n. g_pre f_sys i n)"
 
@@ -798,24 +228,6 @@ proof
   show "f 0 \<union> (\<Union>n. f (Suc n)) \<subseteq> \<Union> (range f)" by auto
 qed
 
-(*lemma "(\<Union>n. eval (g_pre f_sys i (Suc n)) s)
-    \<subseteq> eval (subst (f_sys ! i) (\<lambda>i. if i < length f_sys then g f_sys i else V i)) s"
-proof
-  fix x
-  assume "x \<in> (\<Union>n. eval (g_pre f_sys i (Suc n)) s)"
-  then obtain n where n_intro: "x \<in> eval (g_pre f_sys i (Suc n)) s" by auto
-
-  let ?s_g_pre = "\<lambda>j. if j < length f_sys then eval (g_pre f_sys j n) s else s j"
-  let ?s_g = "\<lambda>j. if j < length f_sys then eval (g f_sys j) s else s j"
-  have s_g_pre_subseteq_s_g: "?s_g_pre j \<subseteq> ?s_g j" for j unfolding g_def by auto
-
-  from n_intro have "x \<in> eval (f_sys ! i) ?s_g_pre"
-    using g_pre_eval[of f_sys ?s_g_pre] by auto
-  with s_g_pre_subseteq_s_g have "x \<in> eval (f_sys ! i) ?s_g"
-    using lfun_mono_aux[of ?s_g_pre ?s_g] by auto
-  then show "x \<in> eval (subst (f_sys ! i) (\<lambda>i. if i < length f_sys then g f_sys i else V i)) s"
-    using substitution_lemma by (smt (verit) eval.simps(1))
-qed*)
 
 lemma g_pre_g_Union: "(\<Union>n. eval (g_pre f_sys i (Suc n)) s) =
   eval (subst (f_sys ! i) (\<lambda>i. if i < length f_sys then g f_sys i else V i)) s"
@@ -843,6 +255,7 @@ proof -
   finally show ?thesis .
 qed
 
+
 lemma solves_f_if_solves_g_eq:
   assumes "\<forall>i < length f_sys. eval (g f_sys i) s = s i"
   shows "solves_eq_sys f_sys s"
@@ -858,6 +271,7 @@ unfolding solves_eq_sys_def proof (standard, standard)
 qed
 
 
+(* The lemma from Pilling's paper *)
 lemma lemma_paper:
   assumes "\<forall>eq \<in> set f_sys. regular_fun eq"
     shows "\<exists>g_sys. length g_sys = length f_sys \<and> indep_ub g_sys (length f_sys - 1)
@@ -881,8 +295,18 @@ proof -
   from length_g_sys indep_g_sys g_sol_of_f f_sol_of_g show ?thesis by blast
 qed
 
+end
+
+
 
 section \<open>The theorem from the paper\<close>
+
+subsection \<open>Special representation of regular functions\<close>
+
+(* We first show that for every regular function f there is a representation of the form
+   (3) (see Pilling's paper, we call it regular_fun' in the following)
+   that has the same parikh image as f
+*)
 
 definition regular_fun' :: "nat \<Rightarrow> 'a lfun \<Rightarrow> bool" where
   "regular_fun' x f \<equiv> \<exists>p q. regular_fun p \<and> regular_fun q \<and>
@@ -898,6 +322,9 @@ lemma epsilon_regular: "regular_fun (N {[]})"
   using lang.simps(2) by blast
 
 
+(* Every regular function can be represented in form (3),
+   as long as we only care for the Parikh image
+*)
 lemma regular_fun_regular_fun': "regular_fun f \<Longrightarrow>
     \<exists>f'. regular_fun' x f' \<and> (\<forall>s. parikh_img (eval f s) = parikh_img (eval f' s))"
 proof (induction rule: regular_fun.induct)
@@ -1020,6 +447,12 @@ next
 qed
 
 
+
+subsection \<open>Minimal solution\<close>
+
+(* We show that F(E)*E (in the following q(p)*p is a minimal solution) *)
+
+(* F(E)*E is a regular function *)
 lemma g_star_e_is_reg:
   assumes p_reg:      "regular_fun p"
       and q_reg:      "regular_fun q"
@@ -1035,6 +468,7 @@ proof -
 qed
 
 
+(* F(E)*E is a solution of equation (3) from the paper (with \<supseteq> instead of =) *)
 lemma g_star_e_is_sol_ineq:
   assumes p_reg:      "regular_fun p"
       and q_reg:      "regular_fun q"
@@ -1071,6 +505,7 @@ unfolding partial_sol_ineq_def proof
 qed
 
 
+(* F(E)*E does not contain the variable x *)
 lemma g_star_e_indep:
   assumes p_reg:      "regular_fun p"
       and q_reg:      "regular_fun q"
@@ -1084,6 +519,7 @@ proof -
 qed
 
 
+(* F(E)*E is the minimal solution *)
 lemma g_star_e_is_minimal:
   assumes p_reg:      "regular_fun p"
       and q_reg:      "regular_fun q"
@@ -1117,6 +553,7 @@ proof -
 qed
 
 
+(* F(E)*E solves equation (3) from the paper (this time with =) *)
 lemma g_star_e_is_sol_eq:
   assumes p_reg:      "regular_fun p"
       and q_reg:      "regular_fun q"
@@ -1153,6 +590,7 @@ unfolding partial_sol_eq_def proof
 qed
 
 
+(* Given equation (3), there exists a regular minimal solution *)
 lemma exists_minimal_reg_sol_aux:
   assumes p_reg: "regular_fun p"
       and q_reg: "regular_fun q"
@@ -1176,6 +614,7 @@ unfolding partial_min_reg_sol_eq_def proof
 qed
 
 
+(* Given equation (2), there exists a regular minimal solution *)
 lemma exists_minimal_reg_sol:
   assumes f_reg: "regular_fun f"
   shows "\<exists>sol. partial_min_reg_sol_eq x f sol"
@@ -1236,11 +675,15 @@ proof -
   then show ?thesis unfolding partial_min_reg_sol_eq_def by blast
 qed
 
+
+(* Unfortunately, the proof is incomplete
+   An proof by induction will prove the theorem in Pilling's paper
+*)
+
+(* solve each equation step by step, reducing the variables one by one *)
 lemma exists_minimal_reg_sol_sys:
   assumes eqs_reg:    "\<forall>eq \<in> set sys. regular_fun eq"
       and r_valid:    "r \<le> length sys"
-   (*   and eqs_indep:  "\<forall>i<r. (\<forall>y \<in> vars (sys ! i). y \<ge> r)" *)
-   (*   and i_valid:    "i < r"  *)
     shows             "\<exists>sols. (\<forall>i<r. partial_min_reg_sol_eq i (sys ! i) (sols i)
                               \<and> (\<forall>i\<ge>r. sols i = V i) \<and> (\<forall>y \<in> vars (sols i). y \<ge> r))"
 using assms proof (induction r)
@@ -1255,7 +698,6 @@ using assms proof (induction r)
     let ?eq' = "subst (sys ! r) sols"
     from sols_reg Suc.prems(2) have "regular_fun ?eq'"
       by (simp add: Suc_le_lessD eqs_reg subst_reg_fun)
-    then obtain "partial_min_reg_sol_eq x f sol"
     show "\<exists>sol_r. partial_min_reg_sol_eq r (sys ! r) sol_r \<and> (\<forall>y\<in>vars sol_r. y \<ge> Suc r)" sorry
   qed
 
@@ -1263,77 +705,11 @@ using assms proof (induction r)
 qed simp
 
 
- (* shows "\<exists>sol. regular_fun sol \<and> x \<notin> vars sol \<and> partial_sol_eq x f sol
-            \<and> (\<forall>sol'. x \<notin> vars sol' \<and> partial_sol_ineq x f sol'
-                      \<longrightarrow> (\<forall>s. parikh_img (eval sol s) \<subseteq> parikh_img (eval sol' s)))"*)
+(* Now, the partial solutions must be substituted, this time backwards.
+   Unfortunately, this part is missing.
+   The connections to CFGs and the actual Parikh theorem is also missing
+ *)
 
-
-
-
-(* maybe we also need x \<in> vars f or something like this here? *)
-lemma theorem_paper_aux:
-  assumes "regular_fun f"
-  shows "\<exists>h. regular_fun h \<and> partial_sol x f h
-            \<and> (\<forall>h'. partial_sol x f h' \<longrightarrow>
-                (\<forall>s. parikh_img (eval h s) \<subseteq> parikh_img (eval h' s)))"
-  sorry
-
-lemma theorem_paper:
-  assumes "\<forall>eq \<in> set f_sys. regular_fun eq"
-    shows "\<exists>gs. (\<forall>g \<in> set gs. regular_fun g) \<and> partial_sol_sys f_sys gs
-                  \<and> (\<forall>gs'. partial_sol_sys f_sys gs'
-                    \<longrightarrow>(\<forall>s. \<forall>i<length gs. subseteq_comm (eval (gs ! i) s) (eval (gs' ! i) s)))"
-  sorry
-
-lemma
-  assumes "\<forall>eq \<in> set f_sys. regular_fun eq"
-      and "indep_lb f_sys (length f_sys)"
-    shows "\<exists>s. (\<forall>i. regular_lang (s i)) \<and> solves_eq_sys_comm f_sys s
-          \<and> (\<forall>s'. solves_eq_sys_comm f_sys s' \<longrightarrow> (\<forall>i. parikh_img (s' i) \<subseteq> parikh_img (s i)))"
-  sorry
-
-
-lemma lfp_fixpoint:
-  assumes "mono f"
-  shows "f (lfp f) = lfp f"
-  unfolding lfp_def
-proof (rule order_antisym)
-  let ?H = "{u. f u \<le> u}"
-  let ?a = "Inf ?H"
-  show "f ?a \<le> ?a"
-  proof (rule Inf_greatest)
-    fix x
-    assume "x \<in> ?H"
-    then have "?a \<le> x" by (rule Inf_lower)
-    with \<open>mono f\<close> have "f ?a \<le> f x" ..
-    also from \<open>x \<in> ?H\<close> have "f x \<le> x" ..
-    finally show "f ?a \<le> x" .
-  qed
-  show "?a \<le> f ?a"
-  proof (rule Inf_lower)
-    from \<open>mono f\<close> and \<open>f ?a \<le> ?a\<close> have "f (f ?a) \<le> f ?a" ..
-    then show "f ?a \<in> ?H" ..
-  qed
-qed
-
-thm lfp_rolling
-
-lemma testhaha:
-  fixes eq :: "'a lfun"
-  assumes "sol = lfp (\<lambda>s. (\<lambda>y. if x = y then eval eq s else s y))"
-  assumes "sol_parikh = lfp (\<lambda>s. (\<lambda>y. if x = y then parikh_img (eval eq s) else {}))"
-  shows "True"
-
-lemma lfp_rolling2:
-  assumes "mono h" "mono f"
-  shows "h (lfp (\<lambda>x. f (h x))) = lfp (\<lambda>x. h (f x))"
-
-(*
-f \<equiv> (\<lambda>s. eval eq s)
-g \<equiv> (\<lambda>lang. parikh_img lang)
-
-mono f; mono g \<Longrightarrow> parikh_img (lfp (\<lambda>x. f (?g x))) = lfp (\<lambda>x. ?g (?f x))
-*)
 
 
 end
