Parikh/Lfun.thy
@@ -1,0 +1,292 @@
+theory Lfun
+  imports 
+    "$AFP/Regular-Sets/Regular_Set"
+    "$AFP/Regular-Sets/Regular_Exp"
+begin
+
+
+section \<open>Definition of language functions\<close>
+
+(* "language functions" are functions which get languages as arguments and also
+   produce languages.
+*)
+
+datatype 'a lfun = V nat                        (* Variable *)
+                 | N "'a lang"                  (* Constant *)
+                 | Union2 "'a lfun" "'a lfun"
+                 | UnionC "nat \<Rightarrow> 'a lfun"      (* Countable union *)
+                 | Conc "'a lfun" "'a lfun"     (* Concatenation *)
+                 | Star "'a lfun"
+
+(* instantiate each variable with a language *)
+type_synonym 'a state = "nat \<Rightarrow> 'a lang"
+
+(* evaluate function for a given state, this produces a language *)
+primrec eval :: "'a lfun \<Rightarrow> 'a state \<Rightarrow> 'a lang" where
+  "eval (V n) s = s n" |
+  "eval (N l) _ = l" |
+  "eval (Union2 f g) s = eval f s \<union> eval g s" |
+  "eval (UnionC f) s = (\<Union>i. eval (f i) s)" |
+  "eval (Conc f g) s = eval f s @@ eval g s" |
+  "eval (Star f) s = star (eval f s)"
+
+(* all variables occurring in a function *)
+primrec vars :: "'a lfun \<Rightarrow> nat set" where
+  "vars (V n) = {n}" |
+  "vars (N _) = {}" |
+  "vars (Union2 f g) = vars f \<union> vars g" |
+  "vars (UnionC f) = (\<Union>i. vars (f i))" |
+  "vars (Conc f g) = vars f \<union> vars g" |
+  "vars (Star f) = vars f"
+
+(* substitute each occurrence of a variable i by the language function s i *)
+primrec subst :: "'a lfun \<Rightarrow> (nat \<Rightarrow> 'a lfun) \<Rightarrow> 'a lfun" where
+  "subst (V n) s = s n" |
+  "subst (N l) _ = N l" |
+  "subst (Union2 f g) s = Union2 (subst f s) (subst g s)" |
+  "subst (UnionC f) s = UnionC (\<lambda>i. subst (f i) s)" |
+  "subst (Conc f g) s = Conc (subst f s) (subst g s)" |
+  "subst (Star f) s = Star (subst f s)"
+
+
+
+section \<open>Some lemmas about the introduced functions\<close>
+
+lemma substitution_lemma:
+  assumes "\<forall>i. s' i = eval (upd i) s"
+  shows "eval (subst f upd) s = eval f s'"
+  using assms by (induction rule: lfun.induct) auto
+
+
+lemma vars_subst: "vars (subst f upd) = (\<Union>x \<in> vars f. vars (upd x))"
+  by (induction f) auto
+
+lemma vars_subst_upper: "vars (subst f upd) \<subseteq> (\<Union>x. vars (upd x))"
+  using vars_subst by force
+
+
+lemma eval_vars:
+  assumes "\<forall>i \<in> vars f. s i = s' i"
+  shows "eval f s = eval f s'"
+  using assms by (induction f) auto
+
+lemma eval_vars_subst:
+  assumes "\<forall>i \<in> vars f. s i = eval (upd i) s"
+  shows "eval (subst f upd) s = eval f s"
+proof -
+  let ?s' = "\<lambda>i. if i \<in> vars f then s i else eval (upd i) s"
+  let ?s'' = "\<lambda>i. eval (upd i) s"
+  have s'_s'': "?s' i = ?s'' i" for i using assms by simp
+  then have s_s'': "\<forall>i. ?s'' i = eval (upd i) s" by simp
+
+  from assms have "eval f s = eval f ?s'" using eval_vars[of f] by simp
+  also have "\<dots> = eval (subst f upd) s"
+    using assms substitution_lemma[OF s_s'', of f] by (simp add: eval_vars)
+  finally show ?thesis by simp
+qed
+
+
+
+section \<open>Monotonicity of language functions\<close>
+
+lemma lfun_mono_aux:
+  assumes "\<forall>i. s i \<subseteq> s' i"
+    shows "eval f s \<subseteq> eval f s'"
+using assms proof (induction rule: lfun.induct)
+  case (Conc x1a x2a)
+  then show ?case by fastforce
+next
+  case (Star f)
+  then show ?case
+    by (smt (verit, best) eval.simps(6) in_star_iff_concat order_trans subsetI)
+qed auto
+
+lemma lfun_mono:
+  fixes f :: "'a lfun"
+  shows "mono (eval f)"
+  using lfun_mono_aux by (metis le_funD monoI)
+
+
+
+section \<open>Continuity of language functions\<close>
+
+(* Surprisingly, I could not find such a lemma in Regular_Set.thy *)
+lemma langpow_mono:
+  fixes A :: "'a lang"
+  assumes "A \<subseteq> B"
+  shows "A ^^ n \<subseteq> B ^^ n"
+using assms conc_mono[of A B] by (induction n) auto
+
+lemma lfun_cont_aux1:
+  assumes "\<forall>i. s i \<le> s (Suc i)"
+      and "w \<in> (\<Union>i. eval f (s i))"
+    shows "w \<in> eval f (\<lambda>x. \<Union>i. s i x)"
+proof -
+  from assms(2) obtain n where n_intro: "w \<in> eval f (s n)" by auto
+  have "s n x \<subseteq> (\<Union>i. s i x)" for x by auto
+  with n_intro show "?thesis"
+    using lfun_mono_aux[of "s n" "\<lambda>x. \<Union>i. s i x"] by auto
+qed
+
+lemma langpow_Union_eval:
+  assumes "\<forall>i. s i \<le> s (Suc i)"
+      and "w \<in> (\<Union>i. eval f (s i)) ^^ n"
+    shows "w \<in> (\<Union>i. eval f (s i) ^^ n)"
+using assms proof (induction n arbitrary: w)
+  case 0
+  then show ?case by simp
+next
+  case (Suc n)
+  then obtain u v where w_decomp: "w = u@v" and
+    "u \<in> (\<Union>i. eval f (s i)) \<and> v \<in> (\<Union>i. eval f (s i)) ^^ n" by fastforce
+  with Suc have "u \<in> (\<Union>i. eval f (s i)) \<and> v \<in> (\<Union>i. eval f (s i) ^^ n)" by auto
+  then obtain i j where i_intro: "u \<in> eval f (s i)" and j_intro: "v \<in> eval f (s j) ^^ n" by blast
+  let ?m = "max i j"
+  from i_intro Suc.prems(1) lfun_mono_aux have 1: "u \<in> eval f (s ?m)"
+    by (metis le_fun_def lift_Suc_mono_le max.cobounded1 subset_eq)
+  from Suc.prems(1) lfun_mono_aux have "eval f (s j) \<subseteq> eval f (s ?m)"
+    by (metis le_fun_def lift_Suc_mono_le max.cobounded2)
+  with j_intro langpow_mono have 2: "v \<in> eval f (s ?m) ^^ n" by auto
+  from 1 2 show ?case using w_decomp by auto
+qed
+
+lemma lfun_cont_aux2:
+  assumes "\<forall>i. s i \<le> s (Suc i)"
+      and "w \<in> eval f (\<lambda>x. \<Union>i. s i x)"
+    shows "w \<in> (\<Union>i. eval f (s i))"
+using assms proof (induction arbitrary: w rule: lfun.induct)
+  case (Conc f g)
+  then obtain u v where w_decomp: "w = u@v"
+    and "u \<in> eval f (\<lambda>x. \<Union>i. s i x) \<and> v \<in> eval g (\<lambda>x. \<Union>i. s i x)" by auto
+  with Conc have "u \<in> (\<Union>i. eval f (s i)) \<and> v \<in> (\<Union>i. eval g (s i))" by auto
+  then obtain i j where i_intro: "u \<in> eval f (s i)" and j_intro: "v \<in> eval g (s j)" by blast
+  let ?m = "max i j"
+  from i_intro Conc.prems(1) lfun_mono_aux have "u \<in> eval f (s ?m)"
+    by (metis le_fun_def lift_Suc_mono_le max.cobounded1 subset_eq)
+  moreover from j_intro Conc.prems(1) lfun_mono_aux have "v \<in> eval g (s ?m)"
+    by (metis le_fun_def lift_Suc_mono_le max.cobounded2 subset_eq)
+  ultimately show ?case using w_decomp by auto
+next
+  case (Star f)
+  then obtain n where n_intro: "w \<in> (eval f (\<lambda>x. \<Union>i. s i x)) ^^ n"
+    using eval.simps(6) star_pow by blast
+  with Star have "w \<in> (\<Union>i. eval f (s i)) ^^ n" using langpow_mono by blast
+  with Star.prems have "w \<in> (\<Union>i. eval f (s i) ^^ n)" using langpow_Union_eval by auto
+  then show ?case by (auto simp add: star_def)
+qed fastforce+
+
+
+(* The actual continuity lemma *)
+lemma lfun_cont:
+  assumes "\<forall>i. s i \<le> s (Suc i)"
+  shows "eval f (\<lambda>x. \<Union>i. s i x) = (\<Union>i. eval f (s i))"
+proof
+  from assms show "eval f (\<lambda>x. \<Union>i. s i x) \<subseteq> (\<Union>i. eval f (s i))" using lfun_cont_aux2 by auto
+  from assms show "(\<Union>i. eval f (s i)) \<subseteq> eval f (\<lambda>x. \<Union>i. s i x)" using lfun_cont_aux1 by blast
+qed
+
+
+
+section \<open>Regular functions\<close>
+
+(* A regular function is a function which evaluates to a regular language
+   if all of its arguments are regular. This applies to all operations
+   defined for lfun, except the countable union (which is needed for the
+   proof of the lemma in Pilling's paper)
+*)
+
+inductive regular_fun :: "'a lfun \<Rightarrow> bool" where
+  Variable:    "regular_fun (V _)" |
+  Const:       "regular_lang l \<Longrightarrow> regular_fun (N l)" |
+  Union2:      "\<lbrakk> regular_fun f; regular_fun g \<rbrakk> \<Longrightarrow> regular_fun (Union2 f g)" |
+  Conc:        "\<lbrakk> regular_fun f; regular_fun g \<rbrakk> \<Longrightarrow> regular_fun (Conc f g)" |
+  Star:        "regular_fun f \<Longrightarrow> regular_fun (Star f)"
+
+declare regular_fun.intros [intro]
+inductive_cases ConstE [elim]:       "regular_fun (N l)"
+inductive_cases Union2E [elim]:      "regular_fun (Union2 f g)"
+inductive_cases ConcE [elim]:        "regular_fun (Conc f g)"
+inductive_cases StarE [elim]:        "regular_fun (Star f)"
+
+
+(* If all arguments are regular, a regular function evaluates to a regular language *)
+lemma regular_fun_regular:
+  assumes "regular_fun f"
+      and "\<And>n. n \<in> vars f \<Longrightarrow> regular_lang (s n)"
+    shows "regular_lang (eval f s)"
+using assms proof (induction rule: regular_fun.induct)
+  case (Union2 f g)
+  then obtain r1 r2 where "Regular_Exp.lang r1 = eval f s \<and> Regular_Exp.lang r2 = eval g s" by auto
+  then have "Regular_Exp.lang (Plus r1 r2) = eval (Union2 f g) s" by simp
+  then show ?case by blast
+next
+  case (Conc f g)
+  then obtain r1 r2 where "Regular_Exp.lang r1 = eval f s \<and> Regular_Exp.lang r2 = eval g s" by auto
+  then have "Regular_Exp.lang (Times r1 r2) = eval (Conc f g) s" by simp
+  then show ?case by blast
+next
+  case (Star f)
+  then obtain r  where "Regular_Exp.lang r = eval f s" by auto
+  then have "Regular_Exp.lang (Regular_Exp.Star r) = eval (Star f) s" by simp
+  then show ?case by blast
+qed auto
+
+
+(* A regular function stays regular if all variables are substituted by regular functions *)
+lemma subst_reg_fun:
+  assumes "regular_fun f"
+      and "\<forall>x \<in> vars f. regular_fun (upd x)"
+    shows "regular_fun (subst f upd)"
+  using assms by (induction rule: regular_fun.induct) auto
+
+
+(* f(Y*Z, X\<^sub>1, \<dots>, X\<^sub>m) = Y* f(Z, X\<^sub>1, \<dots>, X\<^sub>m) if f is a regular function
+
+  Pilling's paper shows "=", but needs an additional assumption and I don't unterstand how
+  the proof should work in the Union case:
+     if f(Y*Z, X\<^sub>1, \<dots>, X\<^sub>m) = g(Y*Z, X\<^sub>1, \<dots>, X\<^sub>m) \<union> h(Y*Z, X\<^sub>1, \<dots>, X\<^sub>m) and g contains Y*Z, but h doesn't,
+     then g(Y*Z, X\<^sub>1, \<dots>, X\<^sub>m) \<union> h(Y*Z, X\<^sub>1, \<dots>, X\<^sub>m) = Y* (g(Z, X\<^sub>1, \<dots>, X\<^sub>m) \<union> h(Z, X\<^sub>1, \<dots>, X\<^sub>m)) seems
+     wrong to me
+*)
+lemma reg_fun_homogeneous_aux:
+  assumes "regular_fun f"
+      and "s x = star Y @@ Z"
+    shows "eval f s \<subseteq> star Y @@ eval f (s(x := Z))"
+using assms proof (induction rule: regular_fun.induct)
+  case (Variable uu)
+  then show ?case sorry
+next
+  case (Const l)
+  have "eval (N l) s \<subseteq> star Y @@ eval (N l) s" using concI_if_Nil1 by blast
+  then show ?case by simp
+next
+  case (Union2 f g)
+  then show ?case sorry
+next
+  case (Conc f g)
+  then show ?case sorry
+next
+  case (Star f)
+  then show ?case sorry
+qed
+
+
+(* reformulate previous lemma with regular functions as arguments instead of languages *)
+lemma reg_fun_homogeneous:
+  assumes "regular_fun f"
+      and "regular_fun y"
+      and "regular_fun z"
+    shows "eval (subst f (\<lambda>a. if a = x then Conc (Star y) z else V a)) s
+      \<subseteq> eval (Conc (Star y) (subst f (\<lambda>a. if a = x then z else V a))) s" (is "?L \<subseteq> ?R")
+proof -
+  let ?s' = "\<lambda>a. if a = x then star (eval y s) @@ eval z s else s a"
+  have "?L = eval f ?s'"
+    using substitution_lemma[of ?s' "\<lambda>a. if a = x then Conc (Star y) z else V a"] by fastforce
+  also have "\<dots> \<subseteq> star (eval y s) @@ eval f (?s'(x := eval z s))"
+    using assms reg_fun_homogeneous_aux[of f ?s'] by simp
+  also have "\<dots> = ?R" using substitution_lemma[of "?s'(x := eval z s)"] by simp
+  finally show ?thesis .
+qed
+
+
+end
